NLustre/Stream.v
@@ -96,14 +96,14 @@ if the clocked stream is [absent] at the corresponding instant. *)
     | S m, true => S (count rs m)
     end.
 
-  (* (** [mask o k rs xs] is the stream which clips the stream [xs] between *)
-  (*     the [k]th and the [(k+1)]th reset, outputting [o] everywhere else. *) *)
-  (* Definition mask {A} (opaque: A) (k: nat) (rs: cstream) (xs: stream A) : stream A := *)
-  (*   fun n => *)
-  (*     if beq_nat k (count rs n) then xs n else opaque. *)
+  (** [mask o k rs xs] is the stream which clips the stream [xs] between
+      the [k]th and the [(k+1)]th reset, outputting [o] everywhere else. *)
+  Definition mask {A} (opaque: A) (k: nat) (rs: cstream) (xs: stream A) : stream A :=
+    fun n =>
+      if beq_nat k (count rs n) then xs n else opaque.
 
-  Definition masked {A} (k: nat) (rs: cstream) (xs xs': stream A) :=
-    forall n, count rs n = k -> xs' n = xs n.
+  (* Definition masked {A} (k: nat) (rs: cstream) (xs xs': stream A) := *)
+  (*   forall n, count rs n = k -> xs' n = xs n. *)
 
   (** ** Properties *)
 
@@ -160,27 +160,27 @@ if the clocked stream is [absent] at the corresponding instant. *)
     - subst; omega.
   Qed.
 
-  (* Lemma mask_opaque: *)
-  (*   forall {A} (xs: stream A) k r (opaque: A) n, *)
-  (*     count r n <> k -> *)
-  (*     (mask opaque k r xs) n = opaque. *)
-  (* Proof. *)
-  (*   intros ** E. *)
-  (*   unfold mask. *)
-  (*   assert (EqNat.beq_nat k (count r n) = false) as -> *)
-  (*       by (apply EqNat.beq_nat_false_iff; omega); auto. *)
-  (* Qed. *)
+  Lemma mask_opaque:
+    forall {A} (xs: stream A) k r (opaque: A) n,
+      count r n <> k ->
+      (mask opaque k r xs) n = opaque.
+  Proof.
+    intros ** E.
+    unfold mask.
+    assert (EqNat.beq_nat k (count r n) = false) as ->
+        by (apply EqNat.beq_nat_false_iff; omega); auto.
+  Qed.
 
-  (* Lemma mask_transparent: *)
-  (*   forall {A} (xs: stream A) k r (opaque: A) n, *)
-  (*     count r n = k -> *)
-  (*     (mask opaque k r xs) n = xs n. *)
-  (* Proof. *)
-  (*   intros ** E. *)
-  (*   unfold mask. *)
-  (*   assert (EqNat.beq_nat k (count r n) = true) as -> *)
-  (*       by (apply EqNat.beq_nat_true_iff; omega); auto. *)
-  (* Qed. *)
+  Lemma mask_transparent:
+    forall {A} (xs: stream A) k r (opaque: A) n,
+      count r n = k ->
+      (mask opaque k r xs) n = xs n.
+  Proof.
+    intros ** E.
+    unfold mask.
+    assert (EqNat.beq_nat k (count r n) = true) as ->
+        by (apply EqNat.beq_nat_true_iff; omega); auto.
+  Qed.
 
   Add Parametric Morphism : count
       with signature eq_str ==> eq ==> eq
@@ -191,24 +191,24 @@ if the clocked stream is [absent] at the corresponding instant. *)
     now rewrite IHn.
   Qed.
 
-  (* Add Parametric Morphism (A: Type) : (@mask A) *)
-  (*     with signature eq ==> eq ==> eq_str ==> eq_str ==> eq_str *)
-  (*       as mask_eq_str. *)
-  (* Proof. *)
-  (*   intros ** E1 ? ? E2 n; unfold mask. *)
-  (*   now rewrite E1, E2. *)
-  (* Qed. *)
-
-  Add Parametric Morphism (A: Type) : (@masked A)
-      with signature eq ==> eq_str ==> eq_str ==> eq_str ==> Basics.impl
-        as masked_eq_str.
+  Add Parametric Morphism (A: Type) : (@mask A)
+      with signature eq ==> eq ==> eq_str ==> eq_str ==> eq_str
+        as mask_eq_str.
   Proof.
-    unfold masked.
-    intros k r r' Err' x x' Exx' y y' Eyy' M n C.
-    rewrite <-Exx', <-Eyy'.
-    apply M.
-    now rewrite Err'.
+    intros ** E1 ? ? E2 n; unfold mask.
+    now rewrite E1, E2.
   Qed.
+
+  (* Add Parametric Morphism (A: Type) : (@masked A) *)
+  (*     with signature eq ==> eq_str ==> eq_str ==> eq_str ==> Basics.impl *)
+  (*       as masked_eq_str. *)
+  (* Proof. *)
+  (*   unfold masked. *)
+  (*   intros k r r' Err' x x' Exx' y y' Eyy' M n C. *)
+  (*   rewrite <-Exx', <-Eyy'. *)
+  (*   apply M. *)
+  (*   now rewrite Err'. *)
+  (* Qed. *)
 
   Lemma present_injection:
     forall x y, x = y <-> present x = present y.
