NLustre/NLSchedule.v
@@ -307,8 +307,7 @@ Module Type NLSCHEDULE
                        sem_reset G f r xss yss ->
                        sem_reset (schedule G) f r xss yss);
       try (now inversion_clear 1; eauto).
-    - constructor; intro k; specialize (H k); destruct H as (?&?&?).
-      do 2 eexists; intuition eauto.
+    - constructor; intro k; specialize (H k); destruct H; auto.
     - match goal with H:find_node _ _ = _ |- _ =>
                     apply scheduler_find_node in H end.
       econstructor; eauto; destruct n; simpl in *; eauto.
