NLustre/NLSemantics.v
@@ -399,12 +399,8 @@ environment.
     with sem_reset: ident -> stream bool -> stream (list value) -> stream (list value) -> Prop :=
          | SReset:
              forall f r xss yss,
-               (forall k, exists xss' yss',
-                     sem_node f xss' yss'
-                     /\ masked k r xss xss'
-                     /\ masked k r yss yss'
-                     /\ length (xss' 0) = length (xss 0)
-                     /\ length (yss' 0) = length (yss 0)) ->
+               (forall k, sem_node f (mask (all_absent (xss 0)) k r xss)
+                              (mask (all_absent (yss 0)) k r yss)) ->
                sem_reset f r xss yss
 
     with sem_node: ident -> stream (list value) -> stream (list value) -> Prop :=
@@ -474,13 +470,10 @@ enough: it does not support the internal fixpoint introduced by
 
     Hypothesis ResetCase:
       forall f r xss yss,
-        (forall k, exists xss' yss',
-              sem_node G f xss' yss'
-              /\ masked k r xss xss'
-              /\ masked k r yss yss'
-              /\ length (xss' 0) = length (xss 0)
-              /\ length (yss' 0) = length (yss 0)
-              /\ P_node f xss' yss') ->
+        (forall k, sem_node G f (mask (all_absent (xss 0)) k r xss)
+                       (mask (all_absent (yss 0)) k r yss)
+              /\ P_node f (mask (all_absent (xss 0)) k r xss)
+                       (mask (all_absent (yss 0)) k r yss)) ->
         P_reset f r xss yss.
 
     Hypothesis NodeCase:
@@ -516,9 +509,6 @@ enough: it does not support the internal fixpoint introduced by
     Proof.
       - destruct Sem; eauto.
       - destruct Sem as [???? Sem]; eauto.
-        apply ResetCase; intro k; specialize (Sem k);
-          destruct Sem as (? & ? & ? & ? & ? & ?).
-        do 2 eexists; intuition eauto.
       - destruct Sem; eauto.
         eapply NodeCase; eauto.
         induction H7; auto.
@@ -543,41 +533,41 @@ enough: it does not support the internal fixpoint introduced by
             now rewrite H in H')
     end.
 
-  (* Lemma mask_length: *)
-  (*   forall k k' xss r n, *)
-  (*     wf_streams xss -> *)
-  (*     length (mask (all_absent (xss k')) k r xss n) = length (xss n). *)
-  (* Proof. *)
-  (*   intros; unfold mask. *)
-  (*   destruct (EqNat.beq_nat k (count r n)); auto. *)
-  (*   unfold all_absent; rewrite map_length. *)
-  (*   induction k'; induction n; auto. *)
-  (* Qed. *)
+  Lemma mask_length:
+    forall k k' xss r n,
+      wf_streams xss ->
+      length (mask (all_absent (xss k')) k r xss n) = length (xss n).
+  Proof.
+    intros; unfold mask.
+    destruct (EqNat.beq_nat k (count r n)); auto.
+    unfold all_absent; rewrite map_length.
+    induction k'; induction n; auto.
+  Qed.
 
-  (* (** If all masks ar well-formed then the underlying stream of lists *)
-  (*     is well-formed. *) *)
-  (* Lemma wf_streams_mask: *)
-  (*   forall xss r m, *)
-  (*     (forall n, wf_streams (mask (all_absent (xss m)) n r xss)) -> *)
-  (*     wf_streams xss. *)
-  (* Proof. *)
-  (*   unfold wf_streams, mask; intros ** WF k k'. *)
-  (*   pose proof (WF (count r k) k' k) as WFk; *)
-  (*     pose proof (WF (count r k') k' k) as WFk'. *)
-  (*   rewrite <-EqNat.beq_nat_refl in WFk, WFk'. *)
-  (*   rewrite NPeano.Nat.eqb_sym in WFk'. *)
-  (*   destruct (EqNat.beq_nat (count r k) (count r k')); auto. *)
-  (*   now rewrite WFk, <-WFk'. *)
-  (* Qed. *)
+  (** If all masks ar well-formed then the underlying stream of lists
+      is well-formed. *)
+  Lemma wf_streams_mask:
+    forall xss r m,
+      (forall n, wf_streams (mask (all_absent (xss m)) n r xss)) ->
+      wf_streams xss.
+  Proof.
+    unfold wf_streams, mask; intros ** WF k k'.
+    pose proof (WF (count r k) k' k) as WFk;
+      pose proof (WF (count r k') k' k) as WFk'.
+    rewrite <-EqNat.beq_nat_refl in WFk, WFk'.
+    rewrite NPeano.Nat.eqb_sym in WFk'.
+    destruct (EqNat.beq_nat (count r k) (count r k')); auto.
+    now rewrite WFk, <-WFk'.
+  Qed.
 
-  (* Lemma sem_node_wf: *)
-  (*   forall G f xss yss, *)
-  (*     sem_node G f xss yss -> *)
-  (*     wf_streams xss /\ wf_streams yss. *)
-  (* Proof. *)
-  (*   intros ** Sem; split; inv Sem; *)
-  (*     assert_const_length xss; assert_const_length yss; auto. *)
-  (* Qed. *)
+  Lemma sem_node_wf:
+    forall G f xss yss,
+      sem_node G f xss yss ->
+      wf_streams xss /\ wf_streams yss.
+  Proof.
+    intros ** Sem; split; inv Sem;
+      assert_const_length xss; assert_const_length yss; auto.
+  Qed.
 
   (** ** Determinism of the semantics *)
 
@@ -995,8 +985,7 @@ clock to [sem_var_instant] too. *)
       apply IH. intro Hnf. apply Hnin. rewrite Hnf. constructor.
     - intro; eapply SEqFby; eassumption.
     - constructor; intro k.
-      specialize (H k); destruct H as (?&?&?).
-      do 2 eexists; intuition eauto.
+      specialize (H k); destruct H; auto.
     - intro.
       rewrite find_node_tl with (1:=Hnf) in Hf.
       eapply SNode; eauto.
@@ -1049,8 +1038,7 @@ clock to [sem_var_instant] too. *)
                      -> sem_equation (nd::G) bk H eq)
              (P_reset := fun f r xss yss => sem_reset (nd::G) f r xss yss);
       try eauto; try intro HH.
-    - constructor; intro k; specialize (H k); destruct H as (?&?&?).
-      do 2 eexists; intuition eauto.
+    - constructor; intro k; specialize (H k); destruct H; auto.
     - clear HH.
       assert (nd.(n_name) <> f) as Hnf.
       { intro Hnf.
@@ -1133,9 +1121,7 @@ clock to [sem_var_instant] too. *)
           by (intro HH; apply Hninieq; rewrite HH; constructor).
       econstructor; eauto.
       inversion_clear Hreset as [???? Hnode].
-      constructor; intro k; specialize (Hnode k); destruct Hnode as (?&?&?).
-      do 2 eexists; intuition eauto.
-      eapply sem_node_cons; eauto.
+      constructor; intro k; specialize (Hnode k); eauto using sem_node_cons.
     - econstructor; eauto.
   Qed.
 
@@ -1189,31 +1175,31 @@ an absent value *)
   now destruct Hsamexs.
   Qed.
 
-  (* Lemma all_absent_mask: *)
-  (*   forall xs k k' r n, *)
-  (*     wf_streams xs -> *)
-  (*     all_absent (mask (all_absent (xs k')) k r xs n) = all_absent (xs n). *)
-  (* Proof. *)
-  (*   intros ** Wf; unfold mask. *)
-  (*   destruct (EqNat.beq_nat k (count r n)); auto. *)
-  (*   specialize (Wf n k'). *)
-  (*   assert (length (all_absent (xs k')) = length (xs n)) as Length *)
-  (*       by now (unfold all_absent; rewrite map_length). *)
-  (*   clear Wf; revert Length; generalize (xs n) as l, (all_absent (xs k')) as l'. *)
-  (*   induction l, l'; inversion 1; simpl; auto. *)
-  (*   f_equal; auto. *)
-  (* Qed. *)
+  Lemma all_absent_mask:
+    forall xs k k' r n,
+      wf_streams xs ->
+      all_absent (mask (all_absent (xs k')) k r xs n) = all_absent (xs n).
+  Proof.
+    intros ** Wf; unfold mask.
+    destruct (EqNat.beq_nat k (count r n)); auto.
+    specialize (Wf n k').
+    assert (length (all_absent (xs k')) = length (xs n)) as Length
+        by now (unfold all_absent; rewrite map_length).
+    clear Wf; revert Length; generalize (xs n) as l, (all_absent (xs k')) as l'.
+    induction l, l'; inversion 1; simpl; auto.
+    f_equal; auto.
+  Qed.
 
-  (* Lemma absent_list_mask: *)
-  (*   forall xs opaque k r n, *)
-  (*     absent_list (xs n) -> *)
-  (*     absent_list opaque -> *)
-  (*     absent_list (mask opaque k r xs n). *)
-  (* Proof. *)
-  (*   intros ** Abs. *)
-  (*   unfold mask. *)
-  (*   destruct (EqNat.beq_nat k (count r n)); auto. *)
-  (* Qed. *)
+  Lemma absent_list_mask:
+    forall xs opaque k r n,
+      absent_list (xs n) ->
+      absent_list opaque ->
+      absent_list (mask opaque k r xs n).
+  Proof.
+    intros ** Abs.
+    unfold mask.
+    destruct (EqNat.beq_nat k (count r n)); auto.
+  Qed.
 
   Remark all_absent_spec:
     forall A (l: list A),
@@ -1336,12 +1322,7 @@ an absent value *)
     inversion_clear Res as [? ? ? ? Node].
     constructor; intro k.
 
-    specialize (Node k); destruct Node as (?&?&?).
-    do 2 eexists; intuition eauto; try rewrite <-E1.
-    - now rewrite <-E2.
-    - now rewrite <-E3.
-    - now rewrite <-E2.
-    - now rewrite <-E3.
+    specialize (Node k). now rewrite <-E1, <-2 E2, <-2 E3.
   Qed.
 
 End NLSEMANTICS.
